theories/clean_ca.v
@@ -1,0 +1,84 @@
+From mathcomp Require Import all_ssreflect.
+From det Require Import lang run run_prop valid_state elpi elpi_equiv elpi_prop run_prop_hard.
+From elpi.apps Require Import derive derive.std.
+From HB Require Import structures.
+From det Require Import zify_ssreflect.
+
+Fixpoint clean_ca_suffix (bt:alts) (ats: alts) : alts :=
+  match ats with
+  | no_alt => nilC
+  | more_alt (hd,xs) tl => (hd, clean_ca_goals_suffix bt xs) ::: (clean_ca_suffix bt tl)
+  end
+with clean_ca_goals_suffix bt gl :=
+  match gl with
+  | no_goals => nilC 
+  | more_goals hd tl => (clean_ca_G_suffix bt hd) ::: (clean_ca_goals_suffix bt tl)
+  end
+with clean_ca_G_suffix bt g :=
+  match g with
+  | call pr t => call pr t 
+  | cut ca => cut ((take (size ca - size bt) (clean_ca_suffix bt ca)))
+  end.
+
+Lemma clean_ca_suffix_cat {bt L1 L2}:
+  clean_ca_suffix bt (L1 ++ L2) = clean_ca_suffix bt (L1) ++ clean_ca_suffix bt L2.
+Proof. by elim: L1 bt L2 => //= [[s g] gs] IH bt L2; rewrite IH cat_cons. Qed.
+
+Lemma clean_ca_goals_suffix_cat {bt L1 L2}:
+  clean_ca_goals_suffix bt (L1 ++ L2) = clean_ca_goals_suffix bt (L1) ++ clean_ca_goals_suffix bt L2.
+Proof. by elim: L1 bt L2 => //= g gs IH bt L2; rewrite IH cat_cons. Qed.
+
+Lemma clean_ca_add_ca {bt1 L}:
+  clean_ca_suffix bt1 (add_ca_deep bt1 L) = L
+with clean_ca_goals_add_ca_goal bt1 x:
+  clean_ca_goals_suffix bt1 (add_ca_deep_goals bt1 x) = x.
+Proof.
+  - by case: L => /=//-[s1 x] xs/=; rewrite clean_ca_add_ca clean_ca_goals_add_ca_goal.
+  - case: x => /=//g gs; rewrite clean_ca_goals_add_ca_goal.
+    case: g => //= a.
+    congr ((cut _) ::: _).
+    rewrite size_cat addnK clean_ca_suffix_cat clean_ca_add_ca.
+    by rewrite take_size_cat// size_add_ca_deep.
+    Guarded.
+Qed.
+
+Lemma s2l_clean_ca {A s xs bt1}:
+  valid_state A ->
+  state_to_list A s bt1 = xs ->
+     clean_ca_suffix bt1 xs = state_to_list A s nilC.
+Proof.
+  move=> +<- {xs}.
+  elim: A s bt1 => //=.
+  - move=> A HA s B HB s1 bt1.
+    case: ifP => [dA vB|dA /andP[vA bB]]; rewrite !add_ca_deep_empty1.
+      by by rewrite state_to_list_dead//cat0s clean_ca_add_ca.
+    by rewrite !add_ca_deep_cat/= !clean_ca_suffix_cat !clean_ca_add_ca.
+  - move=> A HA B0 HB0 B HB s bt /and5P[_ vA _].
+    case: ifP => /=[sA vB bB0|sA /eqP->{B0 HB0}].
+      rewrite !(success_state_to_list empty vA)//=.
+      move /orPT: bB0 => []bB; last first.
+        by rewrite !(base_and_ko_state_to_list bB)/=!make_lB01_empty2 HB//.
+      have [hd H]:= base_and_state_to_list bB.
+      rewrite !H/= !make_lB01_empty2.
+      rewrite !clean_ca_suffix_cat cats0.
+      set m:= make_lB0 _ _.
+      set n:= make_lB0 _ _.
+
+      admit.
+    case: ifP => [fA bB|fA bB].
+      have:= [elaborate @s2l_size A s bt s nilC].
+      case X: state_to_list => [|[sy y]ys]; case Y: state_to_list => [|[sz z]zs]// _.
+      move /orPT: bB => []bB; last first.
+        by rewrite !(base_and_ko_state_to_list bB)/=.
+      have [hd H]:= base_and_state_to_list bB.
+      rewrite !H/=!H/=.
+      rewrite /make_lB01 cat_cons cat0s clean_ca_goals_suffix_cat.
+      rewrite/make_lB0.
+      admit.
+    have:= [elaborate @s2l_size A s bt s nilC].
+    case X: state_to_list => [|[sy y]ys]; case Y: state_to_list => [|[sz z]zs]// _.
+    have [hd H]:= base_and_state_to_list bB.
+    rewrite !H/=!H/=.
+    rewrite /make_lB01 cat_cons cat0s clean_ca_goals_suffix_cat.
+    admit.
+Admitted.
