theories/clean_ca2.v
@@ -1,0 +1,97 @@
+From mathcomp Require Import all_ssreflect.
+From det Require Import lang run run_prop valid_state elpi elpi_equiv elpi_prop run_prop_hard.
+From elpi.apps Require Import derive derive.std.
+From HB Require Import structures.
+From det Require Import zify_ssreflect.
+
+Fixpoint clean_ca_suffix (pref:alts) (bt:alts) (ats: alts) : alts :=
+  match ats with
+  | no_alt => nilC
+  | more_alt (hd,xs) tl => (hd, clean_ca_goals_suffix pref bt xs) ::: (clean_ca_suffix pref bt tl)
+  end
+with clean_ca_goals_suffix pref bt gl :=
+  match gl with
+  | no_goals => nilC 
+  | more_goals hd tl => (clean_ca_G_suffix pref bt hd) ::: (clean_ca_goals_suffix pref bt tl)
+  end
+with clean_ca_G_suffix pref bt g :=
+  match g with
+  | call pr t => call pr t 
+  | cut ca => cut ((take (size ca - size (pref++bt)) (clean_ca_suffix pref bt ca) ++ if size pref <= size ca then pref else nilC))
+  end.
+
+Lemma clean_ca_suffix_cat {bt pref L1 L2}:
+  clean_ca_suffix pref bt (L1 ++ L2) = clean_ca_suffix pref bt (L1) ++ clean_ca_suffix pref bt L2.
+Proof. by elim: L1 bt L2 => //= [[s g] gs] IH bt L2; rewrite IH cat_cons. Qed.
+
+Lemma clean_ca_goals_suffix_cat {bt pref L1 L2}:
+  clean_ca_goals_suffix pref bt (L1 ++ L2) = clean_ca_goals_suffix pref bt (L1) ++ clean_ca_goals_suffix pref bt L2.
+Proof. by elim: L1 bt L2 => //= g gs IH bt L2; rewrite IH cat_cons. Qed.
+
+Lemma clean_ca_add_ca {bt1 pref L}:
+  clean_ca_suffix pref bt1 (add_ca_deep (pref ++ bt1) (L)) = add_ca_deep pref L
+with clean_ca_goals_add_ca_goal pref bt1 x:
+  clean_ca_goals_suffix pref bt1 (add_ca_deep_goals (pref ++ bt1) x) = add_ca_deep_goals pref x.
+Proof.
+  - by case: L => /=//-[s1 x] xs/=; rewrite clean_ca_add_ca clean_ca_goals_add_ca_goal.
+  - case: x => /=//g gs; rewrite clean_ca_goals_add_ca_goal.
+    case: g => //= a.
+    congr ((cut _) ::: _).
+    rewrite !size_cat addnK.
+    rewrite !size_add_ca_deep !clean_ca_suffix_cat clean_ca_add_ca.
+    rewrite addnC -addnA leq_addr.
+    rewrite take_size_cat//size_add_ca_deep//.
+    Guarded.
+Qed.
+
+Lemma s2l_clean_ca {A s xs pref  bt1}:
+  valid_state A ->
+  state_to_list A s (pref ++ bt1) = xs ->
+     clean_ca_suffix pref bt1 xs = (state_to_list A s pref).
+Proof.
+  move=> +<- {xs}.
+  elim: A s pref bt1 => //=.
+  - move=> s pref bt1; rewrite take0 leqn0; case: pref => //.
+  - move=> A HA s B HB s1 pref bt1.
+    case: ifP => [dA vB|dA /andP[vA bB]].
+      rewrite !add_ca_deep_cat !(state_to_list_dead dA).
+      rewrite clean_ca_suffix_cat cat0s clean_ca_add_ca//.
+    by rewrite !add_ca_deep_cat/= !clean_ca_suffix_cat !clean_ca_add_ca.
+  - move=> A HA B0 HB0 B HB s pref bt /and5P[_ vA _].
+    case: ifP => /=[sA vB bB0|sA /eqP->{B0 HB0}].
+      rewrite !(success_state_to_list empty vA)//=.
+      move /orPT: bB0 => []bB; last first.
+        by rewrite !(base_and_ko_state_to_list bB)/=!make_lB01_empty2 HB//.
+      have [hd H]:= base_and_state_to_list bB.
+      rewrite !H/= !make_lB01_empty2.
+      rewrite !clean_ca_suffix_cat.
+      f_equal.
+      set X := state_to_list (odflt _ _) _.
+      rewrite add_deep_cat.
+      Search add_deep.
+
+      rewrite !clean_ca_suffix_cat cats0.
+      set m:= make_lB0 _ _.
+      set n:= make_lB0 _ _.
+      rewrite !add_ca_deep_cat.
+      rewrite catA.
+
+
+      admit.
+    case: ifP => [fA bB|fA bB].
+      have:= [elaborate @s2l_size A s bt s nilC].
+      case X: state_to_list => [|[sy y]ys]; case Y: state_to_list => [|[sz z]zs]// _.
+      move /orPT: bB => []bB; last first.
+        by rewrite !(base_and_ko_state_to_list bB)/=.
+      have [hd H]:= base_and_state_to_list bB.
+      rewrite !H/=!H/=.
+      rewrite /make_lB01 cat_cons cat0s clean_ca_goals_suffix_cat.
+      rewrite/make_lB0.
+      admit.
+    have:= [elaborate @s2l_size A s bt s nilC].
+    case X: state_to_list => [|[sy y]ys]; case Y: state_to_list => [|[sz z]zs]// _.
+    have [hd H]:= base_and_state_to_list bB.
+    rewrite !H/=!H/=.
+    rewrite /make_lB01 cat_cons cat0s clean_ca_goals_suffix_cat.
+    admit.
+Admitted.
